what a hassle making the pure postcondition of cbor_validate_det work!

src/cbor/pulse/raw/CBOR.Pulse.Raw.Format.Parse.fsti
@@ -22,6 +22,15 @@ val cbor_validate
       else exists v1 v2 . Ghost.reveal v == serialize_cbor v1 `Seq.append` v2 /\ SZ.v res == Seq.length (serialize_cbor v1)
     ))
 
+let cbor_validate_det_post
+  (v: Seq.seq U8.t)
+  (res: SZ.t)
+: Tot prop
+=
+      if SZ.v res = 0
+      then (~ (exists v1 v2 . v == serialize_cbor v1 `Seq.append` v2 /\ R.raw_data_item_ints_optimal v1 /\ R.raw_data_item_sorted deterministically_encoded_cbor_map_key_order v1))
+      else exists v1 v2 . v == serialize_cbor v1 `Seq.append` v2 /\ SZ.v res == Seq.length (serialize_cbor v1) /\ R.raw_data_item_ints_optimal v1 /\ R.raw_data_item_sorted deterministically_encoded_cbor_map_key_order v1
+
 val cbor_validate_det
   (input: slice U8.t)
   (#pm: perm)
@@ -29,9 +38,7 @@ val cbor_validate_det
 : stt SZ.t
     (pts_to input #pm v)
     (fun res -> pts_to input #pm v ** pure (
-      if SZ.v res = 0
-      then (~ (exists v1 v2 . Ghost.reveal v == serialize_cbor v1 `Seq.append` v2 /\ R.raw_data_item_ints_optimal v1 /\ R.raw_data_item_sorted deterministically_encoded_cbor_map_key_order v1))
-      else exists v1 v2 . Ghost.reveal v == serialize_cbor v1 `Seq.append` v2 /\ SZ.v res == Seq.length (serialize_cbor v1) /\ R.raw_data_item_ints_optimal v1 /\ R.raw_data_item_sorted deterministically_encoded_cbor_map_key_order v1
+      cbor_validate_det_post v res
     ))
 
 val cbor_parse
